use sections to define the LTT-PLTT simulation

LTT_PLTT.v
@@ -62,275 +62,270 @@ Proof.
 Qed.
 
 Section SIMULATION.
+  Variable G : LTT.global_env.
+  Variable split : list Component.id.
+  Hypothesis splitWF : split_wf (LTT.get_interfaces G) split.
 
-Theorem initial_states_match:
-  forall Is E EWF split splitWF s,
-    let G := LTT.mkGlobalEnv Is E EWF in
-    LTT.initial_state G s ->
+  Definition G' := PLTT.mkGlobalEnv
+                     (LTT.get_interfaces G)
+                     (LTT.get_entrypoints G) split
+                     (entrypoints_exist_wrt_split G split splitWF)
+                     splitWF.
+
+  Lemma initial_states_match:
+    forall s,
+      LTT.initial_state G s ->
     exists ps,
-      let EWF' := entrypoints_exist_wrt_split G split splitWF in
-      let G' := PLTT.mkGlobalEnv Is E split EWF' splitWF in
       PLTT.initial_state G' ps /\ match_states split s ps.
-Proof.
-  intros Is E EWF split splitWF s G.
-  intros Hinit_s.
-  destruct s as [[[[C d] mem] regs] pc] eqn:Hstate_s.
-  destruct Hinit_s as [C_is_0 [empty_stack [empty_regs main_proc]]].
-  destruct (Util.mem 0 split) eqn:Hcontrol.
-  - exists (PLTT.PC (0, [], mem, regs, EntryPoint.get 0 0 E)).
-    intro G'. split.
-    + unfold PLTT.initial_state.
-      split; auto.
-    + rewrite C_is_0, empty_stack, empty_regs, main_proc. simpl.
-      apply program_control; try auto.
-      * unfold PLTT.is_program_component.
-        apply Util.in_iff_mem_true. auto.
-  - exists (PLTT.CC (0, [], mem)).
-    intro G'. split.
-    + unfold PLTT.initial_state.
-      split; auto.
-    + rewrite C_is_0, empty_stack, empty_regs, main_proc. simpl.
-      apply context_control; try auto.
-      * unfold PLTT.is_context_component.
-        apply Util.not_in_iff_mem_false. auto.
-Qed.
+  Proof.
+    intros s Hs_init.
+    destruct s
+      as [[[[C d] mem] regs] pc] eqn:Hstate_s.
+    destruct Hs_init
+      as [C_is_0 [empty_stack [empty_regs main_proc]]].
+    destruct (Util.mem 0 split) eqn:Hcontrol.
+    - exists (PLTT.PC (0, [], mem, regs,
+                       EntryPoint.get 0 0 (LTT.get_entrypoints G))).
+      split.
+      + unfold PLTT.initial_state.
+        split; auto.
+      + rewrite C_is_0, empty_stack, empty_regs, main_proc. simpl.
+        apply program_control; try auto.
+        * unfold PLTT.is_program_component.
+          apply Util.in_iff_mem_true. auto.
+    - exists (PLTT.CC (0, [], mem)).
+      split.
+      + unfold PLTT.initial_state.
+        split; auto.
+      + rewrite C_is_0, empty_stack, empty_regs, main_proc. simpl.
+        apply context_control; try auto.
+        * unfold PLTT.is_context_component.
+          apply Util.not_in_iff_mem_false. auto.
+  Qed.
 
-Theorem final_states_match:
-  forall s (split : list Component.id),
-    LTT.final_state s ->
-    exists ps, PLTT.final_state ps /\ match_states split s ps.
-Proof.
-  intros s split Hfinal_s.
-  destruct s as [[[[C d] mem] regs] pc] eqn:Hstate_s.
-  destruct Hfinal_s as [empty_stack executing_halt].
-  destruct (Util.mem C split) eqn:Hcontrol.
-  - exists (PLTT.PC (C, [], mem, regs, pc)). split.
-    + split; auto.
-    + subst. apply program_control; auto.
-      * apply Util.in_iff_mem_true. auto.
-  - exists (PLTT.CC (C, [], mem)). split.
-    + split; auto.
-    + subst. apply context_control; auto.
-      * apply Util.not_in_iff_mem_false. auto.
-Qed.
-
-Theorem final_states_match':
-  forall s ps (split : list Component.id),
-    LTT.final_state s ->
-    match_states split s ps ->
-    PLTT.final_state ps.
-Proof.
-  intros s ps split Hs_final Hmatch_states.
-  destruct s as [[[[C d] mem] regs] pc] eqn:Hstate_s.
-  destruct Hs_final as [empty_stack executing_halt].
-  unfold PLTT.final_state.
-  inversion Hmatch_states; subst; auto.
-Qed.
-
-Theorem lockstep_simulation:
-  forall I E s s' t split,
-  (* well-formedness requirements *)
-  forall EWF,
-  forall (splitWF : split_wf I split),
-  forall (memWF : memory_wf I s),
-    (* simulation *)
-    let G := LTT.mkGlobalEnv I E EWF in
-    LTT.step G s t s' ->
-    forall ps,
+  Lemma final_states_match:
+    forall s ps,
+      LTT.final_state s ->
       match_states split s ps ->
-    (exists ps',
-        let EWF' := entrypoints_exist_wrt_split G split splitWF in
-        let G' := PLTT.mkGlobalEnv I E split EWF' splitWF in
-        PLTT.step G' ps t ps' /\ match_states split s' ps').
-Proof.
-  intros I E s s' t split.
-  intros EWF splitWF memWF G Hstep ps Hmatch_states.
+      PLTT.final_state ps.
+  Proof.
+    intros s ps Hs_final Hmatch_states.
+    destruct s
+      as [[[[C d] mem] regs] pc] eqn:Hstate_s.
+    destruct Hs_final
+      as [empty_stack executing_halt].
+    unfold PLTT.final_state.
+    inversion Hmatch_states; subst; auto.
+  Qed.
 
-  (* case analysis on who has control and on the execution *)
-  inversion Hmatch_states as
-      [ C d pd mem pmem regs pc Hcontrol Hpstack Hmem
-      | C d pd mem pmem regs pc Hcontrol Hpstack Hmem ]; subst;
-    inversion Hstep; subst;
+  Lemma lockstep_simulation:
+    forall s t s',
+    forall (memWF : memory_wf (LTT.get_interfaces G) s),
+      LTT.step G s t s' ->
+      forall ps,
+        match_states split s ps ->
+      exists ps',
+        PLTT.step G' ps t ps' /\ match_states split s' ps'.
+  Proof.
+    intros s t s'.
+    intros memWF Hstep ps Hmatch_states.
 
-    (* try to extract the current component memory *)
-    try (destruct (splitWF C Hcontrol) as [CI [C_in_I CI_name]];
-         destruct (memWF CI C C_in_I CI_name) as [Cmem HCmem]);
+    (* useful facts about the global environment *)
+    pose (LTT.get_entrypoints G) as E.
+    pose (LTT.entrypoints_exist G) as EWF.
+    assert (HG_unfolded:
+              G = {|
+                LTT.get_interfaces := LTT.get_interfaces G;
+                LTT.get_entrypoints := LTT.get_entrypoints G;
+                LTT.entrypoints_exist := LTT.entrypoints_exist G
+              |}). {
+      destruct G. simpl. auto.
+    } rewrite HG_unfolded in Hstep.
 
-    (* context epsilon steps (except store) *)
-    try (eexists; split;
-         [ apply PLTT.Context_Epsilon
-         | apply context_control; auto
-         ]);
+    (* case analysis on who has control and on the execution *)
+    inversion Hmatch_states as
+        [ C d pd mem pmem regs pc Hcontrol Hpstack Hmem
+        | C d pd mem pmem regs pc Hcontrol Hpstack Hmem ]; subst;
+      inversion Hstep; subst;
 
-    (* program epsilon steps (except store) *)
-    try (eexists; split;
-         [ eapply PLTT.Program_Epsilon;
-           [ apply HCmem
-           | apply HCmem
-           | eauto
-           | apply Hstep
-           | apply Hmem; auto
-           | apply HCmem
-           ]
-         | auto
-        ]).
+        (* try to extract the current component memory *)
+        try (destruct (splitWF C Hcontrol) as [CI [C_in_I CI_name]];
+             destruct (memWF CI C C_in_I CI_name) as [Cmem HCmem]);
 
-  (* program store *)
-  - exists (PLTT.PC (C, PLTT.to_partial_stack d split,
-                     Memory.set pmem C
-                                (Register.get r1 regs)
-                                (Register.get r2 regs),
-                     regs, pc+1)).
-    split.
-    (* step *)
-    + remember (Memory.local_update
-                  (Register.get r1 regs)
-                  (Register.get r2 regs) Cmem)
-        as updated_Cmem.
-      eapply PLTT.Program_Epsilon with
-        (s:=d) (cmem:=Cmem)
-        (cmem':=updated_Cmem)
-        (wmem':=M.add C updated_Cmem mem).
-      * apply HCmem.
-      * apply M.add_1. reflexivity.
-      * unfold PLTT.maps_match_on.
-        intros. split; intro; eassumption.
-      * unfold Memory.set in Hstep.
-        rewrite (M.find_1 HCmem) in Hstep.
-        rewrite Hequpdated_Cmem.
-        apply Hstep.
-      * apply Hmem; assumption.
-      * unfold Memory.set.
-        apply Hmem in HCmem.
-        rewrite (M.find_1 HCmem).
-        rewrite Hequpdated_Cmem.
-        apply M.add_1.
-        ** reflexivity.
-        ** assumption.
-    (* states match *)
-    + apply program_control; auto.
-      * apply PLTT.update_related_memories with
-          (C:=C) (mem1:=mem) (mem2:=pmem)
-          (addr:=Register.get r1 regs)
-          (val:=Register.get r2 regs);
-          auto.
+        (* context epsilon steps (except store) *)
+        try (eexists; split;
+             [ apply PLTT.Context_Epsilon
+             | apply context_control; auto
+             ]);
 
-  (* program is calling *)
-  - destruct (in_dec Nat.eq_dec C' split) as [ HC'origin | ? ];
-      eexists; split.
-    (* internal call - step *)
-    + apply PLTT.Program_Internal_Call; auto.
-    (* internal call - states match *)
-    + destruct (splitWF C' HC'origin)
-        as [C'I [C'I_in_I C'I_name_is_C']].
-      destruct (EWF C'I C' C'I_in_I C'I_name_is_C')
-        as [C'_in_E' [addrs C'_mapsto_E']].
-      rewrite EntryPoint.get_on_compatible_entrypoints with
-        (E':=E) (addrs:=addrs).
-      apply program_control; eauto.
-      * simpl.
-        apply Util.in_iff_mem_true in Hcontrol.
-        rewrite Hcontrol.
-        reflexivity.
-      * eauto.
-      * auto.
-    (* external call - step *)
-    + apply PLTT.Program_External_Call; auto.
-    (* external call - states match *)
-    + apply context_control; auto.
-      * simpl.
-        apply Util.in_iff_mem_true in Hcontrol.
-        rewrite Hcontrol.
-        reflexivity.
+        (* program epsilon steps (except store) *)
+        try (eexists; split;
+             [ eapply PLTT.Program_Epsilon;
+               [ apply HCmem
+               | apply HCmem
+               | eauto
+               | apply Hstep
+               | apply Hmem; auto
+               | apply HCmem
+               ]
+             | auto
+             ]).
 
-  (* program is returning *)
-  - destruct (in_dec Nat.eq_dec C' split)
-      as [ HC'origin | HC'origin ];
-      eexists; split.
-    (* internal return - step *)
-    + apply PLTT.Program_Internal_Return; auto.
-      * simpl.
-        apply Util.in_iff_mem_true in HC'origin.
-        rewrite HC'origin. reflexivity.
-    (* internal return - states match *)
-    + eauto.
-    (* external return - step *)
-    + apply PLTT.Program_External_Return; auto.
-      * simpl.
-        apply Util.not_in_iff_mem_false in HC'origin.
-        rewrite HC'origin. reflexivity.
-    (* external return - states match *)
-    + eauto.
+    (* program store *)
+    - exists (PLTT.PC (C, PLTT.to_partial_stack d split,
+                       Memory.set pmem C
+                                  (Register.get r1 regs)
+                                  (Register.get r2 regs),
+                       regs, pc+1)).
+      split.
+      (* step *)
+      + remember (Memory.local_update
+                    (Register.get r1 regs)
+                    (Register.get r2 regs) Cmem)
+          as updated_Cmem.
+        eapply PLTT.Program_Epsilon with
+            (s:=d) (cmem:=Cmem)
+            (cmem':=updated_Cmem)
+            (wmem':=M.add C updated_Cmem mem).
+        * apply HCmem.
+        * apply M.add_1. reflexivity.
+        * unfold PLTT.maps_match_on.
+          intros. split; intro; eassumption.
+        * unfold Memory.set in Hstep.
+          rewrite (M.find_1 HCmem) in Hstep.
+          rewrite Hequpdated_Cmem.
+          apply Hstep.
+        * apply Hmem; assumption.
+        * unfold Memory.set.
+          apply Hmem in HCmem.
+          rewrite (M.find_1 HCmem).
+          rewrite Hequpdated_Cmem.
+          apply M.add_1.
+          ** reflexivity.
+          ** assumption.
+      (* states match *)
+      + apply program_control; auto.
+        * apply PLTT.update_related_memories with
+              (C:=C) (mem1:=mem) (mem2:=pmem)
+              (addr:=Register.get r1 regs)
+              (val:=Register.get r2 regs);
+            auto.
 
-  (* context store - states match *)
-  - unfold PLTT.maps_match_on.
-    intros C' C'mem HC'origin.
-    split.
-    + intro HC'map.
-      apply Hmem; auto.
-      * destruct (M.find (elt:=list nat) C mem) eqn:HCfind.
-        ** unfold Memory.set in HC'map.
-           rewrite HCfind in HC'map.
-           apply M.add_3 in HC'map; auto.
-           *** unfold not. intros HeqCC'.
-               apply Hcontrol.
-               rewrite <- HeqCC' in HC'origin.
-               apply HC'origin.
-        ** unfold Memory.set in HC'map.
-           rewrite HCfind in HC'map.
-           assumption.
-    + intro HC'map.
-      assert (HneqCC': C <> C').
-      { intro HeqCC'. apply Hcontrol.
-        rewrite <- HeqCC' in HC'origin. apply HC'origin. }
-      unfold Memory.set.
-      destruct (M.find (elt:=list nat) C mem) eqn:HCfind.
-      * assert (HC'mem: PLTT.M.MapsTo C' C'mem mem).
-        { apply Hmem; assumption. }
-        eapply M.add_2; assumption.
-      * apply Hmem; auto.
+    (* program is calling *)
+    - destruct (in_dec Nat.eq_dec C' split) as [ HC'origin | ? ];
+        eexists; split.
+      (* internal call - step *)
+      + apply PLTT.Program_Internal_Call; auto.
+      (* internal call - states match *)
+      + destruct (splitWF C' HC'origin)
+          as [C'I [C'I_in_I C'I_name_is_C']].
+        destruct (EWF C'I C' C'I_in_I C'I_name_is_C')
+          as [C'_in_E' [addrs C'_mapsto_E']].
+        rewrite EntryPoint.get_on_compatible_entrypoints with
+            (E':=E) (addrs:=addrs).
+        apply program_control; eauto.
+        * simpl.
+          apply Util.in_iff_mem_true in Hcontrol.
+          rewrite Hcontrol.
+          reflexivity.
+        * eauto.
+        * auto.
+      (* external call - step *)
+      + apply PLTT.Program_External_Call; auto.
+      (* external call - states match *)
+      + apply context_control; auto.
+        * simpl.
+          apply Util.in_iff_mem_true in Hcontrol.
+          rewrite Hcontrol.
+          reflexivity.
 
-  (* context call is calling *) 
-  - destruct (in_dec Nat.eq_dec C' split) as [ HC'origin | ? ];
-      eexists; split.
-    (* external call - step *)
-    + apply PLTT.Context_External_Call;
-        try assumption.
-      * apply PLTT.push_by_context_preserves_partial_stack; eauto.
-    (* external call - states match *)
-    + destruct (splitWF C' HC'origin)
-        as [CI [CI_in_I CI_name_is_C']].
-      destruct (EWF CI C' CI_in_I CI_name_is_C')
-        as [C'_in_E' [addrs C'_mapsto_E']].
-      rewrite EntryPoint.get_on_compatible_entrypoints with
-        (E':=E) (addrs:=addrs).
-      apply program_control; eauto.
-      * eauto.
-      * assumption.
-    (* internal call - step *)
-    + apply PLTT.Context_Internal_Call;
-        try assumption.
-      * apply PLTT.push_by_context_preserves_partial_stack; eauto.
-    (* internal call - states match *)
-    + eauto.
+    (* program is returning *)
+    - destruct (in_dec Nat.eq_dec C' split)
+        as [ HC'origin | HC'origin ];
+        eexists; split.
+      (* internal return - step *)
+      + apply PLTT.Program_Internal_Return; auto.
+        * simpl.
+          apply Util.in_iff_mem_true in HC'origin.
+          rewrite HC'origin. reflexivity.
+      (* internal return - states match *)
+      + eauto.
+      (* external return - step *)
+      + apply PLTT.Program_External_Return; auto.
+        * simpl.
+          apply Util.not_in_iff_mem_false in HC'origin.
+          rewrite HC'origin. reflexivity.
+      (* external return - states match *)
+      + eauto.
 
-  (* context is returning *)
-  - destruct (in_dec Nat.eq_dec C' split) as [HC'origin | ?];
-      eexists; split.
-    (* external return - step*)
-    + apply PLTT.Context_External_Return; auto.
-      * simpl. apply Util.in_iff_mem_true in HC'origin.
-        rewrite HC'origin.
-        reflexivity.
-    (* external return - states match *)
-    + eauto.
-    (* internal return - step *)
-    + apply PLTT.Context_Internal_Return; auto.
-      * apply PLTT.push_by_context_preserves_partial_stack; auto.
-    (* internal return - states match *)
-    + eauto.
-Qed.
+    (* context store - states match *)
+    - unfold PLTT.maps_match_on.
+      intros C' C'mem HC'origin.
+      split.
+      + intro HC'map.
+        apply Hmem; auto.
+        * destruct (M.find (elt:=list nat) C mem) eqn:HCfind.
+          ** unfold Memory.set in HC'map.
+             rewrite HCfind in HC'map.
+             apply M.add_3 in HC'map; auto.
+             *** unfold not. intros HeqCC'.
+                 apply Hcontrol.
+                 rewrite <- HeqCC' in HC'origin.
+                 apply HC'origin.
+          ** unfold Memory.set in HC'map.
+             rewrite HCfind in HC'map.
+             assumption.
+      + intro HC'map.
+        assert (HneqCC': C <> C').
+        { intro HeqCC'. apply Hcontrol.
+          rewrite <- HeqCC' in HC'origin. apply HC'origin. }
+        unfold Memory.set.
+        destruct (M.find (elt:=list nat) C mem) eqn:HCfind.
+        * assert (HC'mem: PLTT.M.MapsTo C' C'mem mem).
+          { apply Hmem; assumption. }
+          eapply M.add_2; assumption.
+        * apply Hmem; auto.
 
+    (* context call is calling *)
+    - destruct (in_dec Nat.eq_dec C' split) as [ HC'origin | ? ];
+        eexists; split.
+      (* external call - step *)
+      + apply PLTT.Context_External_Call;
+          try assumption.
+        * apply PLTT.push_by_context_preserves_partial_stack; eauto.
+      (* external call - states match *)
+      + destruct (splitWF C' HC'origin)
+          as [CI [CI_in_I CI_name_is_C']].
+        destruct (EWF CI C' CI_in_I CI_name_is_C')
+          as [C'_in_E' [addrs C'_mapsto_E']].
+        rewrite EntryPoint.get_on_compatible_entrypoints with
+            (E':=E) (addrs:=addrs).
+        apply program_control; eauto.
+        * eauto.
+        * assumption.
+      (* internal call - step *)
+      + apply PLTT.Context_Internal_Call;
+          try assumption.
+        * apply PLTT.push_by_context_preserves_partial_stack; eauto.
+      (* internal call - states match *)
+      + eauto.
+
+    (* context is returning *)
+    - destruct (in_dec Nat.eq_dec C' split) as [HC'origin | ?];
+        eexists; split.
+      (* external return - step*)
+      + apply PLTT.Context_External_Return; auto.
+        * simpl. apply Util.in_iff_mem_true in HC'origin.
+          rewrite HC'origin.
+          reflexivity.
+      (* external return - states match *)
+      + eauto.
+      (* internal return - step *)
+      + apply PLTT.Context_Internal_Return; auto.
+        * apply PLTT.push_by_context_preserves_partial_stack; auto.
+      (* internal return - states match *)
+      + eauto.
+  Qed.
 End SIMULATION.
 
 End LTT_TO_PLTT.
